<section xmlns:xi="http://www.w3.org/2001/XInclude" xml:id="s_multiple_integrals_applications">
  <title>Applications of multiple integrals</title>
<subsection xml:id="ss_center_of_mass">
  <title>Center of mass</title>
  <idx><h>mass</h><h>of soli</h></idx>
  <definition xml:id="d_center_of_mass">
    <title>Center of mass</title>
    <statement>
      <p>
      Let <m>\mathcal{R}\subseteq \R^n</m> (<m>n=2,3</m>) represent a solid object, and suppose the function <m>\delta\colon\mathcal{R}\rightarrow \R</m> defines the mass density per unit area (<m>n=2</m>) or unit volume (<m>n=3</m>) at points in <m>\mathcal{R}</m>. We define the <term>mass</term>, <term>first moments</term>, and <term>center of mass</term> of <m>\mathcal{R}</m> as follows.
      </p>
      <md>
        <mrow>n =2 </mrow>
        <mrow> \text{Mass: } M\amp=\iint\limits_\mathcal{R}\delta(x,y)\, dA </mrow>
        <mrow> \text{First moments}\colon  M_{y}\amp=\iint\limits_\mathcal{R}x\delta(x,y)\, dA
        \amp  M_{x}\amp=\iint\limits_\mathcal{R}y\delta(x,y)\, dA </mrow>
        <mrow> \text{Center of mass}\colon (\overline{x},\overline{y})\amp=\frac{1}{M}(M_y, M_x) </mrow>
        <mrow>n =3 </mrow>
        <mrow> \text{Mass: } M\amp=\iiint\limits_\mathcal{R}\delta(x,y,z)\, dV </mrow>
        <mrow> \text{First moments}\colon  M_{yz}\amp=\iiint\limits_\mathcal{R}x\delta(x,y,z)\, dV
        \amp  M_{xz}\amp=\iiint\limits_\mathcal{R}y\delta(x,y,z)\, dV
        \amp  M_{xy}\amp=\iiint\limits_\mathcal{R}z\delta(x,y,z)\, dV</mrow>
        <mrow> \text{Center of mass}\colon (\overline{x},\overline{y},\overline{z})\amp=\frac{1}{M}(M_{yz}, M_{xz}, M_{xy}) </mrow>
      </md>.
      When the mass density function <m>\delta</m> is a constant function (<ie />, <m>\delta(x_1,x_2,\dots, x_n)=c</m> for fixed <m>c\in \R</m>), we call the center of mass of <m>\mathcal{R}</m> its <term>centroid</term>. Equivalently, the centroid of <m>\mathcal{R}</m> is its center of mass, assuming <m>\delta=1</m> everywhere.
    </statement>
  </definition>
  <example>
    <title>Centroids of triangles</title>
    <statement>
      <p>
        Let <m>T</m> be the solid triangular region with vertices <m>(0,0),(1,0),(0,1)</m>.
      </p>
      <ol>
        <li>
          <p>
            Compute the center of mass of <m>T</m> when the density function <m>\delta(x,y)=c</m> is constant. (In other words, compute the centroid of <m>T</m>).
          </p>
        </li>
          <li>
            <p>
              Compute the center of mass of <m>T</m> when the density function is given by <m>\delta(x,y)=x+y</m>.
            </p>
        </li>
        <li>
          <p>
            Let <m>T'</m> be the solid triangular region with vertices <m>(0,0),(a,b),(c,d)</m>. Give a formula for the centroid of <m>T'</m> in terms of <m>a,b,c,d</m>.
          </p>
        </li>
      </ol>
    </statement>
    <solution>
      <ol>
        <li>
          <p>
            We compute
            <md>
              <mrow> M \amp = \iint\limits_Tc\, dA </mrow>
              <mrow>  \amp =c\operatorname{area} T=\frac{c}{2}</mrow>
              <mrow> M_y \amp=\iint\limits_T cx\, dA </mrow>
              <mrow> \amp=c\int_0^1\int_0^{1-x}x\, dy\, dx </mrow>
              <mrow>  \amp = c\left(\frac{1}{2}x-\frac{1}{3}x^3\right)\Bigr\vert_0^1</mrow>
              <mrow>  \amp = \frac{c}{6}</mrow>
              <mrow> M_x \amp =\iint\limits_T cy\, dA </mrow>
              <mrow>  \amp =c\int_0^1\int_0^{1-y}y\, dx\, dy</mrow>
              <mrow>  \amp =\frac{c}{6} </mrow>
              <mrow> (\overline{x},\overline{y}) \amp=(M_y/M, M_x/M) </mrow>
              <mrow>  \amp = (1/3,1/3))</mrow>
            </md>.
          Note: intuitively it is no surprise that the center of mass of <m>T</m> lies along the line <m>y=x</m>, since this is an axis of symmetry of <m>T</m>. To make this symmetry argument rigorous, however, requires some finessing.
          </p>
        </li>
        <li>
          <p>
            We compute
            <md>
              <mrow>M \amp = \iint\limits_T x+y\, dA </mrow>
              <mrow> \amp=\int_0^1\int_0^{1-x}x+y\, dy\, dx </mrow>
              <mrow>  \amp =\int_0^1x(1-x)+\frac{1}{2}(1-x)^2\, dx</mrow>
              <mrow>  \amp = \frac{1}{3}</mrow>
              <mrow> M_y  \amp =\iint\limits_T x(x+y)\, dA</mrow>
              <mrow>  \amp = \int_0^1\int_0^{1-x}x^2+xy\, dy\, dx</mrow>
              <mrow>  \amp = \int_0^1x^2(1-x)+\frac{1}{2}x(1-x)^2\, dx</mrow>
              <mrow>  \amp = \frac{1}{8}</mrow>
              <mrow> M_x \amp = \iint\limits_T y(x+y)\, dA </mrow>
              <mrow>  \amp =\int_0^1\int_0^{1-y}xy+y^2\, dx\, dy</mrow>
              <mrow>  \amp =\frac{1}{8}</mrow>
              <mrow> (\overline{x},\overline{y}) \amp=(M_y/M, M_x/M) </mrow>
              <mrow>  \amp = (3/8, 3/8)</mrow>
            </md>.
            Again, it is no surprise that the center of mass lies along the line <m>y=x</m>, since both <m>T</m> and the density function <m>\delta(x,y)=x+y</m> are symmetric with respect to this line. In contrast to the previous computation, the center of mass is further from the origin. This makes sense in terms of our <q>balancing point</q> interpretation of center of mass: in this case the greater amount of mass in the upper right of the triangle moves the balancing point up and to the right.
          </p>
        </li>
        <li>
          <p>
            The transformation <m>G(u,v)=(au+cv, bu+dv)</m> maps the triangle <m>T</m> with vertices <m>(0,0),(1,0), (0,1)</m> in the <m>uv</m>-plane to the given triangle <m>T'</m> in the <m>xy</m>-plane. We can use substitution to reduce the computation for <m>T'</m> to that of <m>T</m>. Let <m>M, M_y, M_x</m> be the mass and moments of <m>T</m>, and <m>M', M_y', M_x'</m> the mass and moments of <m>T'</m>.
            <md>
              <mrow> M'\amp=\iint\limits_{T'}1\, dA </mrow>
              <mrow> \amp =\iint\limits_T \abs{J(G)}\, dA </mrow>
              <mrow>  \amp =\iint\limits_T\abs{ad-bc}\, dA</mrow>
              <mrow>  \amp =\abs{ad-bc}M</mrow>
              <mrow> M_y' \amp=\iint\limits_{T'}x\, dA </mrow>
              <mrow>  \amp =\iint\limits_T (au+cv) \abs{ad-bc}\, dA</mrow>
              <mrow>  \amp =\abs{ad-bc}(a\iint\limits_Tu\, dA+c\iint\limits_T v\, dA)</mrow>
              <mrow>  \amp =\abs{ad-bc}(aM_y+cM_x)</mrow>
              <mrow> M_x' \amp=\iint\limits_{T'}y\, dA </mrow>
              <mrow>  \amp =\iint\limits_T (bu+dv) \abs{ad-bc}\, dA</mrow>
              <mrow>  \amp =\abs{ad-bc}(b\iint\limits_Tu\, dA+d\iint\limits_T v\, dA)</mrow>
              <mrow>  \amp =\abs{ad-bc}(bM_y+dM_x)</mrow>
              <mrow> (\overline{x}',\overline{y}') \amp = (M_y'/M', M_x'/M') </mrow>
              <mrow>  \amp = \frac{1}{M}(aM_y+cM_x, bM_y+dM_x)</mrow>
              <mrow>  \amp = \frac{1}{3}(a+c,b+d)</mrow>
            </md>.
            Note: looking closely at the penultimate line, we see that
            <me>
              (\overline{x}',\overline{y}')=G(\overline{x}, \overline{y})
            </me>.
            In other words, the center of mass of <m>T'=G(T)</m> is the result of applying <m>G</m> to the center of mass of <m>T</m>! This is a consequence of the fact that <m>G</m> is a <em>linear</em> transformation.
          </p>
        </li>
      </ol>
    </solution>
  </example>
  <example>
    <title>Centroid of hemisphere</title>.
    <statement>
      <p>
        Let <m>D</m> be the solid hemisphere <m>x^2+y^2+z^2\leq 4</m>, <m>z\geq 0</m>. Find the center of mass of <m>D</m> assuming the mass density function is given by <m>\delta(x,y,z)=z</m>.
      </p>
    </statement>
    <solution>
      <p>
        It is inuitively clear from the symmetry of <m>D</m>, as well as the fact that <m>\delta(x,y,z)=z</m> does not depend on <m>x</m> or <m>y</m>, that <m>M_{yz}=M_{xz}=0</m>. In more detail let <m>D=D_1\cup D_2</m> where <m>D_1</m> is the right half of <m>D</m> (<ie />, where <m>x\geq 0</m>), and <m>D_2</m> is the left half. Let <m>f(x,y,z)=x\delta(x,y,z)=xz</m>. The transformation <m>G(x,y,z)=(-x,y,z)</m> maps <m>D_1</m> onto <m>D_2</m>. By substitution we have
        <md>
          <mrow>
          \iiint_{D_2}f(x,y,z)\, dV\amp =\iiint_{D_1}f(-x,y,z)\abs{J(G)}\, dV</mrow>
          <mrow>  \amp =\iiint_{D_1}-xz\, dV</mrow>
          <mrow>  \amp =-\iiint_{D_1}f(x,y,z)\, dV</mrow>
        </md>,
        and thus
        <md>
          <mrow>M_{yz} \amp=\iiint_D xz\, dV </mrow>
          <mrow> \amp=\iiint_{D_1}xz\, dV+\iiint_{D_2}xz\, dV </mrow>
          <mrow>  \amp =\iiint_{D_1}xz\, dV-\iiint_{D_1}xz\, dV=0</mrow>
        </md>.
        A similar argument works to show <m>M_x=0</m>.
      </p>
      <p>To compute the remaining ingredients we will use spherical coordinates. Observe that the solid hemisphere <m>D</m> has spherical description
      <me>
        \{(\rho, \phi,\theta)\colon 0\leq \theta\leq 2\pi, 0\leq \phi\leq \pi/2, 0\leq \rho\leq 2\}
      </me>.
      Now compute:
        <md>
          <mrow>M \amp=\iiint_D \delta(x,y,z)\, dV </mrow>
          <mrow> \amp =\iiint_{D}z\, dV</mrow>
          <mrow>  \amp =\int_0^{2\pi}\int_0^{\pi/2}\int_0^2\rho\cos\phi\cdot \rho^2\sin\phi \amp \text{(spher. subst.)}</mrow>
          <mrow>  \amp = 2\pi \int_0^{\pi/2}\cos\phi\sin\phi\, d\phi\int_0^2\rho^3\, d\rho</mrow>
          <mrow>  \amp =\frac{2}{8}\pi(\sin^2\phi)\vert_0^{\pi/2}(\rho^4)\vert_0^{2}</mrow>
          <mrow>  \amp =\frac{1}{4}\pi 2^4=4\pi</mrow>
          <mrow> M_{xy} \amp =\iiint_D z\delta(x,y,z)\, dV </mrow>
          <mrow> \amp =\iiint_{D}z^2\, dV</mrow>
          <mrow>  \amp =\int_0^{2\pi}\int_0^{\pi/2}\int_0^2\rho^2\cos^2\phi\cdot \rho^2\sin\phi \amp \text{(spher. subst.)}</mrow>
          <mrow>  \amp = 2\pi \int_0^{\pi/2}\cos^2\phi\sin\phi\, d\phi\int_0^2\rho^4\, d\rho</mrow>
          <mrow>  \amp =\frac{2}{15}\pi(-\cos^3\phi)\vert_0^{\pi/2}(\rho^5)\vert_0^{2}</mrow>
          <mrow>  \amp =\frac{2}{15}\pi 2^5=\frac{64}{15}\pi</mrow>
          <mrow> (\overline{x},\overline{y},\overline{z}) \amp = (0,0,M_{xy}/M)</mrow>
          <mrow>  \amp = \left(0,0,\frac{16}{15}\right)</mrow>
        </md>.
      </p>
    </solution>
  </example>
</subsection>
<subsection xml:id="ss_joint_probability_function">
  <title>Probability and density functions</title>
  <definition xml:id="d_random_variable">
    <title>Random variable</title>
    <statement>
      <p>
        Let <m>S</m> be any set, which we will consider to be a sample space. A <term>random variable</term> is a function
        <md>
          <mrow>X\colon S \amp\rightarrow \R </mrow>
          <mrow> s\amp \mapsto X(s)</mrow>
        </md>.
      </p>
    </statement>
  </definition>
  <definition xml:id="d_probability_functions">
    <statement>
      <p>
        Let <m>X, Y</m> be random variables defined on the sample space <m>S</m>.  A <term>joint probability density function</term> for <m>X</m> and <m>Y</m> is a function <m>f\colon \R^2\rightarrow \R</m> satisfying the following properties.
        <ol>
          <li>
            <p>
              <m>f(x,y)\geq 0</m>
            </p>
          </li>
          <li>
            <p>
              <m>\int_{-\infty}^\infty\int_{-\infty}^\infty f(x,y)\, dx\, dy=1</m>
            </p>
          </li>
          <li>
            <p>
              <m>\operatorname{Prob}\left( \{s\in S\colon (X(s),Y(s))\in \mathcal{R}\} \right)=\iint\limits_\mathcal{R}f(x,y)\, dA</m> for any <m>\mathcal{R}\subseteq \R^2</m> over which <m>f</m> is integrable.
            </p>
          </li>
        </ol>
      </p>
    </statement>
  </definition>
  <example>
    <title>Joint probability density function </title>
    <statement>
      <p>
        Verify that the function
        <me>
        f(x,y)=\begin{cases}
          6x^2y\amp (x,y)\in [0,1]\times [0,1]\\
          0\amp (x,y)\notin [0,1]\times [0,1]
        \end{cases}
        </me>
        is a joint probability distribution function.
      </p>
    </statement>
    <solution>
      <p>
        Let <m>R=[0,1]\times [0,1]</m>. It is clear that <m>f(x,y)\geq 0</m> for all <m>(x,y)</m>. Furthermore, we have
          <md>
            <mrow>\iint\limits_{\R^2}f(x,y)\, dA \amp = \iint\limits_{R}f(x,y)\, dA \amp ((x,y)\notin R\implies f(x,y)=0)</mrow>
            <mrow> \amp=\int_0^1\int_0^16x^2y\, dy\, dx </mrow>
            <mrow>  \amp =6\int_0^1x^2\, dx\int_0^1 y\, dy</mrow>
            <mrow>  \amp =6(1/3)(1/2)=1</mrow>
          </md>.
      </p>
    </solution>
  </example>
  <definition xml:id="d_uniformly_distibuted">
    <statement>
      <p>
        Let <m>\mathcal{R}\subseteq\R^2</m> have area <m>A</m>. The random variables <m>X, Y</m> are <term>uniformly distributed</term> over <m>\mathcal{R}</m> if their joint probabiltity disribution function is given by
        <me>
          f(x,y)=\begin{cases}
            \frac{1}{A}\amp \text{if } (x,y)\in \mathcal{R}\\
            0 \amp \text{if } (x,y)\not\in \mathcal{R}
        \end{cases}.
        </me>

      </p>
    </statement>
  </definition>
  <definition xml:id="d_expected_value">
    <title>Expected value</title>
    <statement>
      <p>
        Assume the random variables <m>X,Y</m> on the sample set <m>S</m> have joint probability density function <m>f(x,y)</m>. We define the <term>expected values</term> of <m>X</m> and <m>Y</m>, denoted <m>\mu_X</m> and <m>\mu_Y</m>, as
        <md>
          <mrow>\mu_X\amp= \int_{-\infty}^\infty\int_{-\infty}^\infty x\, f(x,y)\, dx\, dy</mrow>
          <mrow>\mu_Y\amp= \int_{-\infty}^\infty\int_{-\infty}^\infty y\, f(x,y)\, dx\, dy</mrow>
        </md>
      </p>
    </statement>
  </definition>
  <example>
    <title>Joint probability density function </title>
    <statement>
      <p>
        Assume random variables <m>X</m> and <m>Y</m> have joint probability density function
        <me>
        f(x,y)=\begin{cases}
          6x^2y\amp (x,y)\in [0,1]\times [0,1]\\
          0\amp (x,y)\notin [0,1]\times [0,1]
        \end{cases}
        </me>.
        <ol>
          <li>
            <p>
              Compute <m>\mu_X</m> and <m>\mu_Y</m> for any two random variables <m>X</m> and <m>Y</m> with joint probability distribution function <m>f</m>.
            </p>
          </li>
          <li>
            <p>
            Compute the probability that <m>X\geq Y</m>.
            </p>
          </li>
        </ol>
      </p>
    </statement>
    <solution>
      <ol>
        <li>
          <p>
            We compute:
            <md>
              <mrow>\mu_X \amp =\iint\limits_R xf(x,y)\, dA  </mrow>
              <mrow> \amp = \int_0^1\int_0^16x^3y\, dx\, dy </mrow>
              <mrow>  \amp = 6\int_0^1x^3\, dx\int_0^1y\, dy</mrow>
              <mrow>  \amp =6(1/4)(1/2)=3/4 </mrow>
              <mrow>\mu_Y \amp =\iint\limits_R yf(x,y)\, dA  </mrow>
              <mrow> \amp = \int_0^1\int_0^16x^2y^2\, dx\, dy </mrow>
              <mrow>  \amp = 6\int_0^1x^2\, dx\int_0^1y^2\, dy</mrow>
              <mrow>  \amp =6(1/3)(1/3)=2/3</mrow>
            </md>.
          </p>
        </li>
        <li>
          <p>
            Let <m>\mathcal{R}=\{(x,y)\in [0,1]\times[0,1]\colon x\geq y\}</m>. We have
            <md>
              <mrow>\operatorname{Prob}(\{s\in S\colon X(s)\geq Y(s)\}) \amp= \operatorname{Prob}(\{s\in S\colon (X(s),Y(s))\in \mathcal{R}\}) </mrow>
              <mrow> \amp = \iint\limits_\mathcal{R}f(x,y)\, dA \amp (<xref ref="d_probability_functions" text="global"/>) </mrow>
              <mrow>  \amp =\int_0^1\int_0^{x}6x^2y\, dy\, dx </mrow>
              <mrow>  \amp = \int_0^13x^4</mrow>
              <mrow>  \amp =\frac{3}{5}</mrow>
            </md>.
          </p>
        </li>
      </ol>
    </solution>
  </example>
</subsection>

</section>
