<section xmlns:xi="http://www.w3.org/2001/XInclude" xml:id="s_substitution_linear">
  <title>Substitution: general</title>
<introduction>
  <p>
    In this section we provide a generalization of sorts of the substitution technique from single-variable calculus. Recall the set up in that context: given a continuous function <m>f</m> and differentiable function <m>g\colon [a,b]\colon\rightarrow \R</m> we have
    <md>
      <mrow> \int_{g(a)}^{g(b)} f(u)\, du \amp =\int_{a}^{b}f(g(x))g'(x)\, dx \amp \left(\begin{array}{c}u=g(x)\\ du=g'(x)\, dx\end{array}\right)</mrow>
    </md>.
    <xref ref="th_substitution"/> is our generalization of this result to double and triple integrals.
  </p>
</introduction>
<definition xml:id="d_transformation">
  <idx><h>transformation</h></idx>
  <idx><h>continuously differentiable</h></idx>
  <title>Transformations</title>
  <statement>
    <p>
      Let <m>D, D'\subseteq \R^n</m>, where <m>n=2</m> or <m>n=3</m>. A function
      <md>
        <mrow>G\colon D \amp\rightarrow D' </mrow>
        <mrow> (x_1,x_2,\dots, x_n) \amp\mapsto (g_1(x_1,x_2,\dots, x_n),\dots, g_n(x_1,x_2,\dots, x_n)) </mrow>
      </md>
      is a <term>transformation</term> if it satisfies the following properties.
      <ol>
          <li>
            <p>
              <m>G</m> is <xref ref="d_injective_surjective_bijective" text="custom">one-to-one (injective)</xref> on the interior of <m>D</m>.
            </p>
          </li>
          <li>
            <p>
              <m>G(D)=D'</m>: <ie />, <m>G\colon D\rightarrow D'</m> is <xref ref="d_injective_surjective_bijective" text="custom">onto (surjective)</xref>.
            </p>
          </li>
      </ol>
      The function <m>G</m> is <term>continuously differentiable</term> at a point <m>(x_1,x_2,\dots, x_n)\in D</m> if for all <m>1\leq i,j\leq n</m> the partial derivative <m>\partial g_i/\partial x_j</m> is continuous at <m>(x_1,x_2,\dots, x_n)</m>.
    </p>
  </statement>
</definition>
<definition xml:id="d_Jacobian_det">
  <idx><h>determinant</h><h>for <m>n=2,3</m></h></idx>
  <idx><h>Jacobian</h></idx>
  <notation>
    <usage><m>\frac{\partial(g_1,g_2,\dots, g_n)}{\partial(x_1,x_2,\dots, x_n)}</m></usage>
    <description>Jacobian of <m>G=(g_1,g_2,\dots, g_n)</m></description>
  </notation>
  <title>Determinant and Jacobian</title>
  <statement>
    <p>
      Recall that the <term>determinant</term> map on <m>n\times n</m> matrices, denoted <m>\det</m>, is defined in the <m>n=2,3</m> cases as
      <md>
        <mrow> \det\begin{pmatrix}
          a\amp b\\ c\amp d
        \end{pmatrix}\amp=ad-bc </mrow>
        <mrow>\det \begin{pmatrix}a\amp b\amp c\\
        d\amp e\amp f\\ g\amp h\amp i
        \end{pmatrix} \amp =a(ei-gh)-b(di-fg)+c(dh-eg) </mrow>
      </md>.
    Let <m>D, D'\subseteq \R^n</m>, where <m>n=2</m> or <m>n=3</m>. Given a function
    <md>
      <mrow>G\colon D \amp\rightarrow D' </mrow>
      <mrow> (x_1,x_2,\dots, x_n) \amp\mapsto (g_1(x_1,x_2,\dots, x_n),\dots, g_n(x_1,x_2,\dots, x_n)) </mrow>
    </md>
    its Jacobian <m>J(G)=\frac{\partial(g_1,g_2,\dots, g_n)}{\partial(x_1,x_2,\dots, x_n)}</m> is the function defined as follows:
    <md>
      <mrow>J(G)=\frac{\partial(g_1,g_2)}{\partial(x_1,x_2)} \amp=\det \begin{pmatrix}
      \frac{\partial g_1}{\partial x}\amp \frac{\partial g_1}{\partial y}\\
      \frac{\partial g_2}{\partial x}\amp \frac{\partial g_2}{\partial y}
      \end{pmatrix} \amp (n=2)</mrow>
      <mrow> J(G)=\frac{\partial(g_1,g_2,g_3)}{\partial(x_1,x_2,x_3)}\amp=\det
      \begin{pmatrix}
        \frac{\partial g_1}{\partial x}\amp \frac{\partial g_1}{\partial y}\amp \frac{\partial g_1}{\partial z}\\
        \frac{\partial g_2}{\partial x}\amp \frac{\partial g_2}{\partial y}\amp \frac{\partial g_2}{\partial z}\\
        \frac{\partial g_3}{\partial x}\amp \frac{\partial g_3}{\partial y}\amp \frac{\partial g_3}{\partial z}
        \end{pmatrix}
        \amp (n=3)  </mrow>
    </md>
    </p>
  </statement>
</definition>
    <remark xml:id="rm_Jacobian_notation">
  <title>Jacobian notation</title>
  <statement>
    <p>
      To ease notation we will often give names to the outputs of the component functions <m>g_1, g_2, \dots, g_n</m>. For example, given a function of the form <m>G(x,y,z)=(g_1(x,y,z),g_2(x,y,z),g_3(x,y,z))</m> we might write
      <md>
        <mrow> u \amp=g_1(x,y,z) </mrow>
        <mrow> v\amp=g_2(x,y,z) </mrow>
        <mrow> w \amp=g_3(x,y,z) </mrow>
      </md>
      for short, in which case the Jacobian of <m>G</m> is denoted
      <m>
        J(G)=\frac{\partial(u,v,w)}{\partial(x,y,z)}
      </m>.
    </p>
  </statement>
</remark>

<definition xml:id="d_invertible_linear_transformations">
  <title>Invertible linear transformations</title>
  <statement>
    <p>
      Functions of the form
      <md>
        <mrow>G(x,y) \amp = (ax+by, cx+dy)=(u,v) \amp (n=2)</mrow>
        <mrow> H(x,y,z)\amp= (ax+by+cz,dx+ey+fz, gx+hy+iz)=(u,v,w) \amp (n=3)</mrow>
      </md>
      where <m>a,b,c,\dots, g,h,i</m> are fixed constants, are called <term>linear</term>. We can easily compute their Jacobians:
      <md>
        <mrow>\frac{\partial(u,v)}{\partial(x,y)} \amp=\det\begin{pmatrix}
          a\amp b\\ c\amp d
        \end{pmatrix}=ad-bc</mrow>
        <mrow> \frac{\partial(u,v,w)}{\partial(x,y,z)}\amp= \det \begin{pmatrix}a\amp b\amp c\\
        d\amp e\amp f\\ g\amp h\amp i
        \end{pmatrix} =a(ei-gh)-b(di-fg)+c(dh-eg) </mrow>
      </md>.
      In linear algebra you learn that the <m>G</m> and <m>H</m> are one-to-one everywhere if and only if the Jacobians <m>J(G)</m> and <m>J(H)</m> are nonzero. This gives us a convenient family of continuously differentiable transformations, called <term>invertible linear transformations</term>.
    </p>
  </statement>
  <!-- <solution>
    <p>

    </p>
  </solution> -->
</definition>
    <remark xml:id="rm_det_notation">
  <statement>
    <p>
      The textbook's determinant notation looks a lot like absolute value notation: <eg />, it writes <m>\det \begin{pmatrix}
        a\amp b\\ c\amp d
      \end{pmatrix}</m> as <m>\abs{\begin{array}{cc} a\amp b\\ c\amp d\end{array}}</m>. This can lead to confusion in the statement of <xref ref="th_substitution"/>, which involves taking the absolute value of the Jacobian of a function. Accordingly, we will stick with our <m>\det</m> notation.
    </p>
  </statement>
</remark>

<theorem xml:id="th_substitution">
  <title>Substitution</title>
  <statement>
    <p>
      Let <m>D, D'</m> be elementary regions of <m>\R^n</m>, where <m>n=2</m> or <m>n=3</m>. If
      <md>
        <mrow>G\colon D \amp\rightarrow D' </mrow>
        <mrow> (x_1,x_2,\dots, x_n) \amp\mapsto (g_1(x_1,x_2,\dots, x_n),\dots, g_n(x_1,x_2,\dots, x_n)) </mrow>
      </md>
      is a transformation that is continuously differentiable at all points in the interior of <m>D</m>, then
      <mdn>
      <mrow xml:id="eq_subst_2_J"> \iint\limits_{\mathcal{D'}}f(x,y)\, dA \amp =\iint\limits_{\mathcal{D}}f\left(G(x,y)\right)
      \left\vert J(G) \right\vert\, dA
      </mrow>
      <mrow xml:id="eq_subst_2_partial">  \amp =\iint\limits_{\mathcal{D}}f(g_1(x,y),g_2(x,y))
      \left\vert\det \begin{pmatrix}
        \frac{\partial g_1}{\partial x}\amp \frac{\partial g_1}{\partial y}\\
        \frac{\partial g_2}{\partial x}\amp \frac{\partial g_2}{\partial y}
        \end{pmatrix}\right\vert\, dA
      </mrow>,
      </mdn>
      in the <m>n=2</m> case, and
      <mdn>
        <mrow xml:id="eq_subst_3_J"> \iiint\limits_{\mathcal{D'}}f(x,y,z)\, dV \amp =\iiint\limits_{\mathcal{D}}f\left(G(x,y,z)\right)
        \left\vert J(G)\right\vert\, dV
        </mrow>
        <mrow xml:id="eq_subst_3_partial">  \amp =\iiint\limits_{\mathcal{D}}f(g_1(x,y,z),g_2(x,y,z),g_3(x,y,z))
        \left\vert\det \begin{pmatrix}
          \frac{\partial g_1}{\partial x}\amp \frac{\partial g_1}{\partial y}\amp \frac{\partial g_1}{\partial z}\\
          \frac{\partial g_2}{\partial x}\amp \frac{\partial g_2}{\partial y}\amp \frac{\partial g_2}{\partial z}\\
          \frac{\partial g_3}{\partial x}\amp \frac{\partial g_3}{\partial y}\amp \frac{\partial g_3}{\partial z}
          \end{pmatrix}\right\vert\, dV
          </mrow>
      </mdn>,
      in the <m>n=3</m> case.
    </p>
  </statement>
</theorem>
    <remark xml:id="rm_substitution_as_changeofvar">
  <title>Substitution as change of variable</title>
  <statement>
    <p>
      Substitution is often described as a <em>change of variable</em> technique. Let's see why, treating the <m>n=2</m> case. Suppose we are asked to compute <m>\iint\limits_\mathcal{R}f(x,y)\, dA</m> over the region <m>\mathcal{R}'</m>. If we want to make use of <xref ref="eq_subst_2_J"/> to transform this integral to a simpler one, we should treat <m>\mathcal{R}</m> as <m>\mathcal{D'}</m>, the <em>target</em> region in our substitution setup.
    </p>
    <p>
      Next, suppose that in terms of the expressions
      <md>
      <mrow> u \amp = h_1(x,y)</mrow>
      <mrow> v \amp = h_2(x,y)</mrow>
    </md>
    we have <m>f(x,y)=q(h_1(x,y),h_2(x,y))=q(u,v)</m>. Substitution allows us to compute the original integral in terms of an integral involving the new function <m>q</m> as follows:
    <ol>
      <li>
        <p>
          Let <m>H=(h_1(x,y),h_2(x,y))</m>. The function <m>H</m> maps our original region <m>\mathcal{R}</m> to a new region <m>\mathcal{S}</m> that we consider to live in the <m>uv</m>-plane.
        </p>
      </li>
      <li>
        <p>
          Since <m>\mathcal{R}=\mathcal{D}'</m> in the <xref ref="th_substitution"/> setup, we identify <m>\mathcal{S}=\mathcal{D}</m> in this setup.
        </p>
      </li>
      <li>
        <p>
          If <m>H</m> is a <em>transformation</em>, then it is invertible, and there is an inverse function <m>H^{-1}=G=(g_1(u,v),g_2(u,v))</m>, where
          <md>
          <mrow> x \amp = g_1(u,v)</mrow>
          <mrow> y \amp = g_2(u,v)</mrow>
        </md>
        are equations expressing <m>x</m> and <m>y</m> in terms of <m>u</m> and <m>v</m>. By inverse properties, <m>G</m>
        maps <m>\mathcal{S}</m> (in the <m>uv</m>-plane) onto <m>\mathcal{R}</m> (in the <m>xy</m>-plane).
        </p>
      </li>
      <li>
        <p>
        Using <xref ref="th_substitution"/> we have
        <md>
          <mrow>\iint\limits_{\mathcal{R}}f(x,y)\, dA \amp =\iint\limits_{\mathcal{S}}f(g_1(u,v),g_2(u,v))\vert J(G)\vert\,dA </mrow>
          <mrow> \amp = \iint\limits_{\mathcal{S}}q(u,v)\left\vert\frac{\partial(x,y)}{\partial(u,v)}\right\vert\, dA</mrow>
        </md>.
        </p>
      </li>
    </ol>
    </p>
  </statement>
</remark>
<p>
Let's make the discussion above official with a procedure. As above, it is expressed for <m>n=2</m> case, but generalizes easily to <m>n=3</m>.
</p>
<algorithm xml:id="proc_subst_change_of_variable">
  <title>Substitution as change of variable</title>
  <statement>
    <p>
      Suppose <m>f</m> is defined over the region <m>\mathcal{R}\subseteq \R^2</m>, and we have <m>f(x,y)=q(u,v)</m>, where <m>u</m> and <m>v</m> are expressions of the form
      <mdn>
      <mrow xml:id="eqs_change_var1"> u \amp = h_1(x,y)</mrow>
      <mrow xml:id="eqs_change_var2"> v \amp = h_2(x,y)</mrow>
    </mdn>.
    To transform the integral <m>\iint\limits_\mathcal{R}f(x,y)\,dA</m> using the change of variables <xref first="eqs_change_var1" last="eqs_change_var2"/>, proceed as follows.
    <ol>
      <li>
        <p>
          Let <m>H=(h_1,h_2)</m>. Determine the region <m>\mathcal{S}</m> that <m>\mathcal{R}</m> is mapped onto by <m>H</m>: <ie />, compute  <m>\mathcal{S}=H(\mathcal{R})</m>.
        </p>
      </li>
      <li>
        <p>
          We have
          <men xml:id="eq_subst_change_var">
            \iint\limits_{\mathcal{R}}f(x,y)\, dA=\iint\limits_{\mathcal{S}}q(u,v)\left\vert\frac{\partial(x,y)}{\partial(u,v)}\right\vert\, dA
          </men>.
        </p>
      </li>
      <li>
        <p>
          To compute <m>\frac{\partial(x,y)}{\partial(u,v)}</m> you can either:
          <ol>
            <li>
              <p>
                determine the inverse function <m>H^{-1}=G=(g_1,g_2)</m> by solving for <m>x</m> and <m>y</m> in terms of <m>u</m> and <m>v</m> as
                <md>
                <mrow> x \amp = g_1(u,v)</mrow>
                <mrow> y \amp = g_2(u,v)</mrow>
              </md>
              and compute <m>J(G)=\partial(g_1,g_2)/\partial(u,v)</m> directly, or
              </p>
            </li>
            <li>
              <p>assuming <m>H</m> and <m>G</m> are both continuously differentiable,
                compute <m>J(G)</m> <em>indirectly</em>, using the fact that
                <me>
                  J(G)=\frac{1}{J(H)}
                </me>.
                Observe that <m>1/J(H)</m> is an expression in <m>x</m> and <m>y</m> that you will need to express in terms of <m>u</m> and <m>v</m>!
              </p>
            </li>
          </ol>
        </p>
      </li>
    </ol>
    </p>
  </statement>
</algorithm>
<example>
  <title>Substitution: linear, two variables</title>
  <statement>
    <p>
      Define <m>\mathcal{R}</m> be the trapezoid with vertices <m>(0,1),(0,2),(1,0),(2,0)</m>. Use a substitution to compute
      <me>
        \iint\limits_\mathcal{R}e^{(x-y)/(x+y)}\, dA
      </me>

    </p>
  </statement>
  <solution>
    <p>
      Use the substitution <m>H(x,y)</m>
      <md>
        <mrow>u \amp =x-y</mrow>
        <mrow>v \amp =x+y </mrow>
      </md>
      with inverse <m>G(u,v)</m>
      <md>
        <mrow>x\amp=\frac{1}{2}(u+v) </mrow>
        <mrow>y \amp=\frac{1}{2}(-u+v) </mrow>
      </md>
      and Jacobian <m>\partial(x,y)/\partial(u,v)=\frac{1}{2}</m>. The trapezoidal region in the <m>xy</m>-plane has boundary equations <m>x+y=1, x+y=2, x=0, y=0</m>, which are transformed to the boundary equations <m>v=1, v=2, u=-v, u=v</m>. This defines the trapezoidal region
      <me>
        \mathcal{S}=\{(u,v)\colon 1\leq v\leq 2, -v\leq u\leq v\}
      </me>
      in the <m>uv</m>-plane, and by substitution we have
      <md>
        <mrow>\iint\limits_{\mathcal{R}}e^{(x-y)/x+y)}\, dA \amp = \iint\limits_\mathcal{S}e^(u/v)\abs{\frac{\partial(x,y)}{\partial(u,v)}}\, dA </mrow>
        <mrow> \amp=\int_1^2\int_{-v}^v\frac{1}{2}e^(u/v)\, du\, dv</mrow>
        <mrow>  \amp = \frac{1}{2}\int_1^2v(e-1/e)\, dv</mrow>
        <mrow>  \amp =\frac{3}{4}(e-1/e)</mrow>
      </md>

    </p>
  </solution>
</example>
<example>
  <title>Volume of ellipsoid</title>
  <statement>
    <p>
      Let <m>\mathcal{R}</m> be the solid ellipsoid defined by the inequality
      <me>
        \frac{x^2}{a^2}+\frac{y^2}{b^2}+\frac{z^2}{c^2}\leq 1
      </me>,
      where <m>a,b,c\in \R</m> are fixed constants.
      Use change of variables to compute
      <me>
        \operatorname{vol} \mathcal{R}=\iiint\limits_\mathcal{R}1\, dV
      </me>.
    </p>
  </statement>
  <solution>
    <p>
      The transformation <m>G(u,v,w)=(au,bv,cw)</m> transforms the the solid ball <m>\mathcal{S}\colon u^2+v^2+w^2\leq 1</m> in <m>uvw</m>-space to the given ellispoid <m>\mathcal{R}</m> in <m>xyz</m>-space. The Jacobian of <m>G</m> is
      <me>
       J(G)=\det \begin{pmatrix}
          a\amp 0\amp 0\\
          0\amp b\amp 0\\
          0\amp 0\amp c
        \end{pmatrix}=abc
      </me>.
      Now compute
      <md>
        <mrow>\operatorname{vol} \mathcal{R}  \amp =\iiint\limits_\mathcal{R}1\, dV </mrow>
        <mrow> \amp =\iiint\limits_\mathcal{S}1 \abs{J(G)}\, dV \amp \text{(subst.)} </mrow>
        <mrow>  \amp =abc\iiint\limits_\mathcal{S}1\, dV</mrow>
        <mrow>  \amp =abc\operatorname{vol}\mathcal{S}</mrow>
        <mrow>  \amp =\frac{4}{3}\pi abc </mrow>
      </md>,
      since the volume of the unit ball <m>\mathcal{R}</m> is <m>4\pi/3</m>.
    </p>
  </solution>
</example>

</section>
